Blake2s: proof for blak2s_round

code/hash/Hacl.Impl.Blake2s.fst
@@ -77,6 +77,7 @@ type working_vector = lbuffer uint32 16
 type message_block = lbuffer uint32 16
 type hash_state = lbuffer uint32 8
 type idx = n:size_t{size_v n < 16}
+type sigma_t = lbuffer (n:size_t{size_v n < 16}) 160
 
 
 
@@ -124,44 +125,40 @@ let blake2_mixing wv a b c d x y =
 
 #set-options "--max_fuel 0 --z3rlimit 10"
 
-val blake2_round1 : wv:working_vector -> m:message_block -> i:size_t -> sigma:lbuffer (n:size_t{size_v n < 16}) 160 ->
+val blake2_round1 : wv:working_vector -> m:message_block -> i:size_t -> sigma:sigma_t ->
   Stack unit
-    (requires (fun h -> live h wv /\ live h m /\ live h sigma))
+    (requires (fun h -> live h wv /\ live h m /\ live h sigma
+                  /\ as_list h.[sigma] == sigma_list_size))
     (ensures  (fun h0 _ h1 -> preserves_live h0 h1
                          /\ modifies1 wv h0 h1
+                         /\ h0.[m] == h1.[m]
+                         /\ as_list h1.[sigma] == sigma_list_size
                          /\ h1.[wv] == Spec.blake2_round1 h0.[wv] h0.[m] (v i)))
 
 let blake2_round1 wv m i sigma =
   let i_mod_10 = size_mod i (size 10) in
   let start_idx = mul_mod #SIZE i_mod_10 (size 16) in
-  let h0 = ST.get () in
   let s = sub #(n:size_t{v n < 16}) #160 #16 sigma start_idx (size 16) in
-  let h1 = ST.get () in
-  assert(h0 == h1);
-  assert(live h1 sigma);
-  assert(as_lseq s h1 == as_lseq (sub #(n:size_t{v n < 16}) #160 #16 sigma start_idx (size 16)) h1);
-  lemma_sub_live3 #h1 #(n:size_t{v n < 16}) #160 #16 sigma start_idx (size 16) s;
-  // assert(live h1 s);
   blake2_mixing wv (size 0) (size 4) (size  8) (size 12) (m.(s.(size 0))) (m.(s.(size 1)));
   blake2_mixing wv (size 1) (size 5) (size  9) (size 13) (m.(s.(size 2))) (m.(s.(size 3)));
   blake2_mixing wv (size 2) (size 6) (size 10) (size 14) (m.(s.(size 4))) (m.(s.(size 5)));
-  blake2_mixing wv (size 3) (size 7) (size 11) (size 15) (m.(s.(size 6))) (m.(s.(size 7)));
-  admit()
+  blake2_mixing wv (size 3) (size 7) (size 11) (size 15) (m.(s.(size 6))) (m.(s.(size 7)))
 
 
-val blake2_round2 : wv:working_vector -> m:message_block -> i:size_t -> sigma:lbuffer (n:size_t{size_v n < 16}) 160 ->
+val blake2_round2 : wv:working_vector -> m:message_block -> i:size_t -> sigma:sigma_t ->
   Stack unit
-    (requires (fun h -> live h wv /\ live h m /\ live h sigma))
+    (requires (fun h -> live h wv /\ live h m /\ live h sigma
+                   /\ as_list h.[sigma] == sigma_list_size))
     (ensures  (fun h0 _ h1 -> preserves_live h0 h1
                          /\ modifies1 wv h0 h1
+                         /\ h0.[m] == h1.[m]
+                         /\ as_list h1.[sigma] == sigma_list_size
                          /\ h1.[wv] == Spec.blake2_round2 h0.[wv] h0.[m] (v i)))
 
 let blake2_round2 wv m i sigma =
   let i_mod_10 = size_mod i (size 10) in
   let start_idx = mul_mod #SIZE i_mod_10 (size 16) in
   let s = sub #(n:size_t{v n < 16}) #160 #16 sigma start_idx (size 16) in
-  let h = ST.get () in
-  assume(live h s);
   blake2_mixing wv (size 0) (size 5) (size 10) (size 15) (m.(s.(size 8))) (m.(s.(size 9)));
   blake2_mixing wv (size 1) (size 6) (size 11) (size 12) (m.(s.(size 10))) (m.(s.(size 11)));
   blake2_mixing wv (size 2) (size 7) (size  8) (size 13) (m.(s.(size 12))) (m.(s.(size 13)));
@@ -170,7 +167,8 @@ let blake2_round2 wv m i sigma =
 
 val blake2_round : wv:working_vector -> m:message_block -> i:size_t -> sigma:lbuffer (n:size_t{size_v n < 16}) 160 ->
   Stack unit
-    (requires (fun h -> live h wv /\ live h m /\ live h sigma))
+    (requires (fun h -> live h wv /\ live h m /\ live h sigma
+                   /\ as_list h.[sigma] == sigma_list_size))
     (ensures  (fun h0 _ h1 -> preserves_live h0 h1
                          /\ modifies1 wv h0 h1
                          /\ h1.[wv] == Spec.blake2_round h0.[wv] h0.[m] (v i)))
